adjust freeze step

Splinter/AllocationsLayer/AllocationJournal.i.dfy
@@ -49,7 +49,7 @@ module AllocationJournal {
 
   datatype TransitionLabel =
       ReadForRecoveryLabel(messages: MsgHistory)
-    | FreezeForCommitLabel(frozenJournal: JournalImage, unobserved: set<AU>)
+    | FreezeForCommitLabel(frozenJournal: JournalImage)
     | QueryEndLsnLabel(endLsn: LSN)
     | PutLabel(messages: MsgHistory)
     | DiscardOldLabel(startLsn: LSN, requireEnd: LSN, deallocs: set<AU>)
@@ -64,7 +64,7 @@ module AllocationJournal {
     function I(): LikesJournal.TransitionLabel {
       match this {
         case ReadForRecoveryLabel(messages) => LikesJournal.ReadForRecoveryLabel(messages)
-        case FreezeForCommitLabel(frozenJournal, _) => LikesJournal.FreezeForCommitLabel(frozenJournal.tj)
+        case FreezeForCommitLabel(frozenJournal) => LikesJournal.FreezeForCommitLabel(frozenJournal.tj)
         case QueryEndLsnLabel(endLsn) => LikesJournal.QueryEndLsnLabel(endLsn)
         case PutLabel(messages) => LikesJournal.PutLabel(messages)
         case DiscardOldLabel(startLsn, requireEnd, _) => LikesJournal.DiscardOldLabel(startLsn, requireEnd)
@@ -112,7 +112,6 @@ module AllocationJournal {
     && v.WF()
     && lbl.FreezeForCommitLabel?
     && step.FreezeForCommitStep?
-    && lbl.unobserved == v.UnobservedAUs()
 
     && LikesJournal.FreezeForCommit(v.journal, v'.journal, lbl.I(), step.depth)
     && v' == v.(
