Splinter/AllocationsLayer/CoordinationJournal.i.dfy
@@ -21,9 +21,10 @@ module CoordinationJournal {
     | ReadForRecoveryLabel(records: MsgHistory)
     | QueryEndLsnLabel(endLsn: LSN)
     | PutLabel(records: MsgHistory)
+    | FreezeAsLabel(unobserved: set<AU>)
     | InternalLabel(allocs: set<AU>, deallocs: set<AU>)
     | QueryLsnPersistenceLabel(syncLsn: LSN)
-    | CommitStartLabel(newBoundaryLsn: LSN, maxLsn: LSN, unobserved: set<AU>)
+    | CommitStartLabel(newBoundaryLsn: LSN, maxLsn: LSN)
     | CommitCompleteLabel(requireEnd: LSN, discarded: set<AU>)
     | CrashLabel()
 
@@ -118,6 +119,16 @@ module CoordinationJournal {
     && v' == v
   }
 
+  predicate FreezeUnobserved(v: Variables, v': Variables, lbl: TransitionLabel)
+  {
+    && v.WF()
+    && lbl.FreezeAsLabel?
+    && v.ephemeral.Known?
+    && v.inFlight.None?
+    && lbl.unobserved == v.ephemeral.v.UnobservedAUs()
+    && v' == v
+  }
+
   predicate CommitStart(v: Variables, v': Variables, lbl: TransitionLabel)
   {
     && v.WF()
@@ -131,7 +142,7 @@ module CoordinationJournal {
 
     && var frozenJournal := v'.inFlight.value;
     && AllocationJournal.Next(v.ephemeral.v, v'.ephemeral.v, 
-      AllocationJournal.FreezeForCommitLabel(frozenJournal, lbl.unobserved))
+      AllocationJournal.FreezeForCommitLabel(frozenJournal))
 
     // Frozen journal stitches to frozen map
     && frozenJournal.tj.SeqStart() == lbl.newBoundaryLsn
@@ -189,7 +200,8 @@ module CoordinationJournal {
       case PutLabel(_) => Put(v, v', lbl)
       case InternalLabel(_, _) => Internal(v, v', lbl)
       case QueryLsnPersistenceLabel(_) => QueryLsnPersistence(v, v', lbl)
-      case CommitStartLabel(_, _, _) => CommitStart(v, v', lbl)
+      case FreezeAsLabel(_) => FreezeUnobserved(v, v', lbl)
+      case CommitStartLabel(_, _) => CommitStart(v, v', lbl)
       case CommitCompleteLabel(_, _) => CommitComplete(v, v', lbl)
       case CrashLabel() => Crash(v, v', lbl)
     }
